Given a list of strings  `words`  and a string  `pattern`, return  _a list of_  `words[i]`  _that match_  `pattern`. You may return the answer in  **any order**.

A word matches the pattern if there exists a permutation of letters  `p`  so that after replacing every letter  `x`  in the pattern with  `p(x)`, we get the desired word.

Recall that a permutation of letters is a bijection from letters to letters: every letter maps to another letter, and no two letters map to the same letter.

**Example 1:**
```
**Input:** words = ["abc","deq","mee","aqq","dkd","ccc"], pattern = "abb"
**Output:** ["mee","aqq"]
**Explanation:** "mee" matches the pattern because there is a permutation {a -> m, b -> e, ...}. 
"ccc" does not match the pattern because {a -> c, b -> c, ...} is not a permutation, since a and b map to the same letter.
```

**Example 2:**
```
**Input:** words = ["a","b","c"], pattern = "a"
**Output:** ["a","b","c"]
```

**Constraints:**

- `1 <= pattern.length <= 20`
- `1 <= words.length <= 50`
- `words[i].length == pattern.length`
- `pattern`  and  `words[i]`  are lowercase English letters.


### Python
```python
class Solution:
    def n(self, pattern):
        data = {}
        result = []
        for p in pattern:
            data[p] = data.get(p, len(data) + 1)
            result.append(data[p])
        return result
    
    def findAndReplacePattern(self, words: List[str], pattern: str) -> List[str]:
        p_arr = self.n(pattern)
        return filter(lambda word: self.n(word) == p_arr, words) 
```

```python
class Solution:
    def findAndReplacePattern(self, words: List[str], pattern: str) -> List[str]:
        def match(word):
            m, n = {}, {}
            for w, p in zip(word, pattern):
                if w not in m:
                    m[w] = p
                if p not in n:
                    n[p] = w
                if (m[w], n[p]) != (p, w):
                    return False
            return True
        
        return filter(match, words)
```